Step 4 or Argon2i spec implemented

specs/Spec.Argon2i.fst
@@ -20,10 +20,10 @@ let h a_len a nn =
 
 val step1 :
   p_len:size_nat -> p : lbytes p_len ->
-  s_len:size_nat{s_len >= 8} -> s: lbytes s_len ->
-  lanes:nat{lanes >= 1 /\ lanes <= pow2 24 - 1} -> t_len:size_nat{t_len >= 4} ->
-  m:size_nat{m >= (8 * lanes)} ->
-  iterations:size_nat{iterations >= 1}  ->
+  s_len:size_nat -> s: lbytes s_len ->
+  lanes:size_nat -> t_len:size_nat ->
+  m:size_nat ->
+  iterations:size_nat ->
   x_len:size_nat -> x:lbytes x_len ->
   k_len:size_nat{k_len + p_len + s_len + x_len + 11*4 <= max_size_t - 2 * Spec.Blake2b.bytes_in_block} -> k:lbytes k_len ->
   Tot (lbytes 64)
@@ -68,7 +68,7 @@ let compute_variable_length_output_size (t_len:size_nat{t_len + 64 <= size_of_bl
     let r = (ceil_32 t_len) - 2 in
     32 * r + 64
 
-val h' : t_len:size_nat{t_len >= 4 /\ t_len <= size_of_block - 64} -> x_len:size_nat{x_len + 4 <= max_size_t - 2 * Spec.Blake2b.bytes_in_block} -> x:lbytes x_len -> Tot (lbytes ( compute_variable_length_output_size t_len))
+val h' : t_len:size_nat{1 <= t_len /\ t_len + 64 <= size_of_block} -> x_len:size_nat{x_len + 4 <= max_size_t - 2 * Spec.Blake2b.bytes_in_block} -> x:lbytes x_len -> Tot (lbytes ( compute_variable_length_output_size t_len))
 
 
 let h' t_len x_len x =
@@ -91,28 +91,69 @@ let h' t_len x_len x =
     in
     update_slice output (r * 32) ((r*32)+64) vlast
 
-
 let fill_block (d_len: size_nat{d_len <= size_of_block}) (d: lbytes d_len) : Tot (lbytes size_of_block) =
   let output = create size_of_block (u8 0) in
   update_slice output 0 d_len d
 
+#reset-options "--z3rlimit 50 --max_fuel 1"
 
-val step3 : t_len:size_nat{t_len >= 4 /\ t_len <= size_of_block - 64} -> lanes:size_nat{lanes >= 1 /\ lanes <= pow2 24 - 1} -> number_of_blocks:size_nat{number_of_blocks * size_of_block <= max_size_t} -> mem_size:size_nat{mem_size= (number_of_blocks + 1) * size_of_block} -> mem: lbytes mem_size -> h0:lbytes 64 -> Tot (lbytes mem_size)
+let block_offset (lanes:size_nat{lanes <> 0}) (columns:size_nat{columns <> 0 /\ columns*lanes*size_of_block <= max_size_t}) (i:size_nat{i<lanes}) (j:size_nat{j<columns}) : Tot (result:size_nat{result <= (lanes * columns - 1) * size_of_block}) =
+   assert (columns * i <= columns * (lanes - 1));
+   assert (columns * i + j <= columns * (lanes - 1) + (columns - 1));
+   assert (columns * i + j <= columns * lanes - 1);
+   size_of_block * (columns * i + j)
 
-let step3 t_len lanes number_of_blocks mem_size mem h0 =
+val step3 : t_len:size_nat{1 <= t_len /\ t_len <= size_of_block - 64} -> lanes:size_nat{lanes >= 1 /\ lanes <= pow2 24 - 1} -> columns:size_nat{1 <= columns /\ lanes * columns * size_of_block <= max_size_t} -> mem: lbytes (lanes * columns * size_of_block) -> h0:lbytes 64 -> Tot (lbytes (lanes * columns * size_of_block))
+
+let step3 t_len lanes columns mem h0 =
   repeati lanes (fun i mem ->
-    let offset: size_nat = (number_of_blocks / lanes) * size_of_block * i in
-    let argument = create (64 + 4 + 4) (u8 0) in
+    let offset: size_nat = block_offset lanes columns i 0 in
+    let argument_length : size_nat = 64 + 4 + 4 in
+    let argument = create argument_length (u8 0) in
     let argument = update_slice argument 0 64 h0 in
-    let argument = update_slice argument (64 + 4) (64 + 4 + 4) (uint_to_bytes_le (u32 i)) in
-    let slice =  fill_block (compute_variable_length_output_size t_len) (h' t_len (64 + 4 + 4) argument) in
+    let argument = update_slice argument (64 + 4) argument_length (uint_to_bytes_le (u32 i)) in
+    let slice =
+      fill_block (compute_variable_length_output_size t_len) (h' t_len argument_length argument)
+    in
     update_slice mem offset (offset + size_of_block) slice
   ) mem
+
+
+val step4 : t_len:size_nat{1 <= t_len /\ t_len <= size_of_block - 64} -> lanes:size_nat{lanes >= 1 /\ lanes <= pow2 24 - 1} -> columns:size_nat{4 <= columns /\ lanes * columns * size_of_block <= max_size_t} -> mem: lbytes (lanes * columns * size_of_block) -> h0:lbytes 64 -> Tot (lbytes (lanes * columns * size_of_block))
+
+let step4 t_len lanes columns mem h0 =
+  repeati lanes (fun i mem ->
+    let offset: size_nat = block_offset lanes columns i 1 in
+    let argument_length : size_nat = 64 + 4 + 4 in
+    let argument = create argument_length (u8 0) in
+    let argument = update_slice argument 0 64 h0 in
+    let argument = update_slice argument 64 68 (uint_to_bytes_le (u32 1)) in
+    let argument = update_slice argument (64 + 4) argument_length (uint_to_bytes_le (u32 i)) in
+    let slice =
+      fill_block (compute_variable_length_output_size t_len) (h' t_len argument_length argument)
+    in
+    update_slice mem offset (offset + size_of_block) slice
+  ) mem
+
+val step5 : t_len:size_nat{1 <= t_len /\ t_len <= size_of_block - 64} -> lanes:size_nat{lanes >= 1 /\ lanes <= pow2 24 - 1} -> columns:size_nat{4 <= columns /\ lanes * columns * size_of_block <= max_size_t} -> mem: lbytes (lanes * columns * size_of_block) -> Tot (lbytes (lanes * columns * size_of_block))
+
+let step5 t_len lanes columns mem =
+  repeati lanes (fun i mem ->
+    repeati (columns-1) (fun j mem ->
+      let j = j + 1 in
+      let offset = block_offset lanes columns i j in
+      let first_block = sub mem (block_offset lanes columns i (j-1)) size_of_block in
+      let second_block = sub mem (block_offset lanes colmuns i j (*TODO*)) size_of_block in
+      let slice = create size_of_block (u8 0) (*TODO*)  in
+      update_slice mem offset (offset+ size_of_block) slice
+    )
+  ) mem
+
 
 val argon2i :
   p_len:size_nat -> p : lbytes p_len ->
   s_len:size_nat{s_len >= 8} -> s: lbytes s_len ->
-  lanes:size_nat{lanes >= 1 /\ lanes <= pow2 24 - 1} -> t_len:size_nat{t_len >= 4 /\ t_len <= max_size_t - 64} ->
+  lanes:size_nat{lanes >= 1 /\ lanes <= pow2 24 - 1} -> t_len:size_nat{t_len >= 4 /\ t_len <= size_of_block - 64} ->
   m:size_nat{m >= (8 * lanes) /\ (m + 4 * lanes)  * 1024 <= max_size_t} ->
   iterations:size_nat{iterations >= 1}  ->
   x_len:size_nat{x_len + 4 <= max_size_t - 2 * Spec.Blake2b.bytes_in_block} -> x:lbytes x_len ->
@@ -122,8 +163,11 @@ val argon2i :
 let argon2i p_len p s_len s lanes t_len m iterations x_len x k_len k =
   let h0 = step1 p_len p s_len s lanes t_len m iterations x_len x k_len k in
   let four_lanes = 4 * lanes in
-  let number_of_blocks = four_lanes * (m / four_lanes) in
+  let columns = 4 * (m / four_lanes) in
+  let number_of_blocks = lanes * columns in
   let memory_size : size_nat = size_of_block * number_of_blocks in
   let memory = create memory_size (u8 0) in
-
+  assert (memory_size = columns * lanes * size_of_block);
+  let memory = step3 t_len lanes columns memory h0 in
+  let memory = step4 t_len lanes columns memory h0 in
   create t_len (u8 0)
